## Iterative Method
**Solve:** T(n) = 3T(n/4) + n for n >= 4  
T(n) = 1 for n < 4  
Move *n* to the left; T(n) = n + 3T(n/4)  

**Substitute in T(n/4) and keep exponents**  
T(n) = n + 3[n/4+3T(n/16)]  
T(n) = (3/4)^0\*n + (3/4)^1\*n + 9T(n/16)  

**AGAIN**  
T(n) = (3/4)^0\*n + (3/4)^1\*n + (3/4)^2\*n + 27T(n/64)  

**Once you recognize the pattern, put in the base case**  
Let k = log4(n), or n = 4^k  

T(n) = (3/4)^0\*n + (3/4)^1\*n + ... + 3^kT(n/4^k)  

FOR THE LAST TERM, IT BECOMES 3^kT(4^k/4^k) = 3^kT(1)  

SO T(n) = (SUM from 0 to k - 1 (3/4)^i\*n) + 3^k  

T(n) = (SUM from 0 to k - 1 (3/4)^i\*n) + 3^(log4(n))  

T(n) = (SUM from 0 to k - 1 (3/4)^i\*n) + n^(log4(3))  

T(n) â‰ˆ 4n + n^.8  

T(n) = Theta(n)  
