## Master Method Simplified
**Assuming recurrence T(n) = aT(n/b) + f(n)**  
With prior assumptions (a >= 1, b > 1, f(n) asymptotically
positive)  
With f(n) = cn^k for c >= 0 and k >= 0  
T(n) = aT(n/b) + cn^k  

IF a > b^k then T(n) = THETA(n^(logb(a)))  
IF a = b^k then T(n) = THETA(n^k\*lg(n))  
IF a < b^k then T(n) = THETA(n^k)  

### Master Method Examples
#### CASE 1
T(n) = 16T(n/4) + n  
a = 16, b = 4, k = 1  
Simplified case 1!  
T(n) = THETA(n^(logb(a))) = THETA(n^log4(16)) = THETA(n^2)  

#### Case 2
T(n) = T(3n/7) + 1  
a = 1, b = 7/3, k = 0  
Simplified case 2!  
T(n) = THETA(n^(logb(a))lg(n)) = THETA(n^k\*lg(n)) = THETA(lg(n))  

#### Case 3
T(n) = 3T(n/2) + n^2  
a = 3, b = 2, k = 2  
Simplified case 3!  
T(n) = THETA(n^k) = THETA(n^2)  

### Simplification
If each right-side T term has the same coefficient:  
Add the coefficients to give a and take the average of the
coefficients inside T to give b  

T(n) = T(n/3) + T(2n/3) + n
